code/streaming/Hacl.Streaming.SHA2.fst
@@ -103,6 +103,7 @@ let free_256 = F.free hacl_sha2_256 (G.hide ()) (state_t_256.s ()) (G.erased uni
 "Hash `input`, of len `input_len`, into `dst`, an array of 32 bytes."]
 val sha256: Hacl.Hash.Definitions.hash_st SHA2_256
 let sha256 input input_len dst =
+  [@inline_let]
   let dst: lbuffer uint8 (Hacl.Hash.Definitions.hash_len SHA2_256) = dst in
   let ib = ntup1 input in
   let rb = ntup1 dst in
@@ -134,6 +135,7 @@ let free_224: F.free_st hacl_sha2_256 (G.hide ()) (state_t_256.s ()) (G.erased u
 "Hash `input`, of len `input_len`, into `dst`, an array of 28 bytes."]
 val sha224: Hacl.Hash.Definitions.hash_st SHA2_224
 let sha224 input input_len dst =
+  [@inline_let]
   let dst: lbuffer uint8 (Hacl.Hash.Definitions.hash_len SHA2_224) = dst in
   let ib = ntup1 input in
   let rb = ntup1 dst in
@@ -182,6 +184,7 @@ let free_512 = F.free hacl_sha2_512 (G.hide ()) (state_t_512.s ()) (G.erased uni
 "Hash `input`, of len `input_len`, into `dst`, an array of 64 bytes."]
 val sha512: Hacl.Hash.Definitions.hash_st SHA2_512
 let sha512 input input_len dst =
+  [@inline_let]
   let dst: lbuffer uint8 (Hacl.Hash.Definitions.hash_len SHA2_512) = dst in
   let ib = ntup1 input in
   let rb = ntup1 dst in
@@ -213,6 +216,7 @@ let free_384: F.free_st hacl_sha2_512 (G.hide ()) (state_t_512.s ()) (G.erased u
 "Hash `input`, of len `input_len`, into `dst`, an array of 48 bytes."]
 val sha384: Hacl.Hash.Definitions.hash_st SHA2_384
 let sha384 input input_len dst =
+  [@inline_let]
   let dst: lbuffer uint8 (Hacl.Hash.Definitions.hash_len SHA2_384) = dst in
   let ib = ntup1 input in
   let rb = ntup1 dst in
