lib/Lib.Sequence.Lemmas.fsti
@@ -442,6 +442,21 @@ val repeat_blocks_split:
       (repeat_blocks_multi blocksize (Seq.slice inp 0 len0) f acc0))
 
 ///
+val repeat_blocks_multi_extensionality:
+    #a:Type0
+  -> #b:Type0
+  -> blocksize:size_pos
+  -> inp:seq a{length inp % blocksize = 0}
+  -> f:(lseq a blocksize -> b -> b)
+  -> g:(lseq a blocksize -> b -> b)
+  -> init:b ->
+  Lemma
+  (requires
+    (forall (block:lseq a blocksize) (acc:b). f block acc == g block acc))
+  (ensures
+    repeat_blocks_multi blocksize inp f init ==
+    repeat_blocks_multi blocksize inp g init)
+
 ///  Properties related to the map_blocks combinator
 ///
 
